disjunctive normal form

chapter-2/Part_5.thy
@@ -31,6 +31,27 @@ fun eval :: "exp \<Rightarrow> int \<Rightarrow> int" where
 
 fun evalp :: "int list \<Rightarrow> int \<Rightarrow> int" where
 "evalp [] n = 0" |
-"evalp (x#xs) n = x * n ^ (size xs) + evalp xs n"
+"evalp (x#xs) n = x + n * evalp xs n"
 
-(* TODO *)
+fun list_sum :: "int list \<Rightarrow> int list \<Rightarrow> int list" where
+"list_sum [] xs = xs" |
+"list_sum xs [] = xs" |
+"list_sum (x#xs) (y#ys) = (x + y) # list_sum xs ys"
+
+fun scalar_mult :: "int \<Rightarrow> int list \<Rightarrow> int list" where
+"scalar_mult n [] = []" |
+"scalar_mult n (x#xs) = n*x # scalar_mult n xs"
+
+fun list_mult :: "int list \<Rightarrow> int list \<Rightarrow> int list" where
+"list_mult [] xs = xs" |
+"list_mult (x#xs) ys = list_sum (scalar_mult x ys) (0 # list_mult xs ys)"
+
+fun coeffs :: "exp \<Rightarrow> int list" where
+"coeffs Var = [0, 1]" |
+"coeffs (Const n) = [n]" |
+"coeffs (Add a b) = list_sum (coeffs a) (coeffs b)" |
+"coeffs (Mult a b) = list_mult (coeffs a) (coeffs b)"
+
+lemma "evalp (coeffs e) x = eval e x"
+  nitpick
+  oops
